\item[(c)]
\section{Transfer Function}

\subsection*{Problem Statement}
Compute the transfer function \( H(z) = \frac{Y(z)}{X(z)} \).

\subsection*{Theoretical Background}
The transfer function \( H(z) \) of a system characterizes its input-output relationship in the z-domain. It is obtained by taking the z-transform of the difference equation and solving for \( H(z) = \frac{Y(z)}{X(z)} \).

\subsection*{Mathematical Derivation}
Given the difference equation:
\[ y[n] = x[n] - \frac{1}{15} y[n-1] + \frac{2}{5} y[n-2] \]

Taking the z-transform of both sides:
\[ Y(z) = X(z) - \frac{1}{15} Y(z) z^{-1} + \frac{2}{5} Y(z) z^{-2} \]

Rearranging to solve for \( \frac{Y(z)}{X(z)} \):
\[ Y(z) + \frac{1}{15} Y(z) z^{-1} - \frac{2}{5} Y(z) z^{-2} = X(z) \]
\[ Y(z) \left( 1 + \frac{1}{15} z^{-1} - \frac{2}{5} z^{-2} \right) = X(z) \]
\[ H(z) = \frac{Y(z)}{X(z)} = \frac{1}{1 + \frac{1}{15} z^{-1} - \frac{2}{5} z^{-2}} \]

Multiplying the numerator and denominator by \( z^2 \) to get a standard form:
\[ H(z) = \frac{z^2}{z^2 + \frac{1}{15} z - \frac{2}{5}} \]

\subsection*{Conclusion}
The transfer function \( H(z) \) of the system is:
\[ H(z) = \frac{z^2}{z^2 + \frac{1}{15} z - \frac{2}{5}} \]
This transfer function characterizes the input-output relationship of the given difference equation in the z-domain.
