%! Author = wolfram_e_laube
%! Date = 02.04.24

\item [a)]
Given the cosine wave expressed as
$$
x(t) = \hat{X} \cos(2\pi f_0 t),
$$
we aim to prove its Fourier transform pair. Using Euler's formula, $\cos(\theta) = \frac{e^{j\theta} + e^{-j\theta}}{2}$, we can express the cosine function as a sum of complex exponentials:
$$
x(t) = \hat{X} \left( \frac{e^{j2\pi f_0 t} + e^{-j2\pi f_0 t}}{2} \right) = \frac{\hat{X}}{2} e^{j2\pi f_0 t} + \frac{\hat{X}}{2} e^{-j2\pi f_0 t}.
$$

The Fourier transform of a complex exponential function is given by:
$$
e^{j2\pi f_0 t} \leftrightarrow \delta(f-f_0)
$$
and
$$
e^{-j2\pi f_0 t} \leftrightarrow \delta(f+f_0).
$$

Therefore, applying the Fourier transform to $x(t)$, we obtain:
$$
X(f) = \frac{\hat{X}}{2} \delta(f-f_0) + \frac{\hat{X}}{2} \delta(f+f_0),
$$
proving the given Fourier transform pair for the cosine wave.

